Remove old substitution and clean up namespaces

LambdaGraph/Nest.lean
@@ -22,20 +22,20 @@ The nesting relation between functions in a program.
 During substitution, all functions nested in the function corresponding to the
 substitution variable must be rewritten.
 -/
-inductive Nests (p : Program) (n : Nat) : Nat → Prop where
+inductive Program.Nests (p : Program) (n : Nat) : Nat → Prop where
   | free (m : Nat) (_ : m < p.size) : n ≠ m → p.fn[m].Free p n → Nests p n m
   | step (m k : Nat) (_ : k < p.size) :
     m ≠ k → p.fn[k].Free p m → Nests p n m → Nests p n k
 
-notation:40 n:41 " ≻[" p:min "] " m:41 => Nests p n m
+notation:40 n:41 " ≻[" p:min "] " m:41 => Program.Nests p n m
 notation:40 n:41 " ⊁[" p:min "] " m:41 => ¬n ≻[p] m
 
 /-- The reflexive closure of the nesting relation. -/
-inductive NestsEq (p : Program) (n : Nat) : Nat → Prop where
+inductive Program.NestsEq (p : Program) (n : Nat) : Nat → Prop where
   | refl (_ : n < p.size) : NestsEq p n n
   | nests (m : Nat) : Nests p n m → NestsEq p n m
 
-notation:40 n:41 " ≽[" p:min "] " m:41 => NestsEq p n m
+notation:40 n:41 " ≽[" p:min "] " m:41 => Program.NestsEq p n m
 notation:40 n:41 " ⋡[" p:min "] " m:41 => ¬n ≽[p] m
 
 /--
@@ -81,28 +81,17 @@ Free variables of a computation.
 A variable occurs free in a computation if it occurs free in the computation's
 expression.
 -/
-def Computation.Free (p : Computation) (n : Nat) := p.expr.Free p.toProgram n
+def Computation.Free (c : Computation) (n : Nat) := c.expr.Free c.toProgram n
 
 /-- A computation is closed if its expression is closed in its program. -/
-def Computation.Closed (p : Computation) : Prop := ∀ n, ¬p.Free n
+def Computation.Closed (c : Computation) : Prop := c.expr.Closed c.toProgram
 
 @[simp]
-theorem not_closed_var {p : Program} {n : Nat} : ¬(Expr.var n).Closed p :=
+theorem Expr.not_closed_var {p : Program} {n : Nat} : ¬(Expr.var n).Closed p :=
   fun h => h n .var
 
-theorem fn_closed_iff {p : Program} {m : Nat} :
-    (Expr.fn m).Closed p ↔ ∀ n ≠ m, (_ : m < p.size) → ¬p.fn[m].Free p n := by
-  constructor
-  · intro hc n hn _
-    intro hne
-    solve_by_elim
-  · intro hf n hn
-    cases hn with
-    | fn _ _ hne hn =>
-      solve_by_elim
-
 @[simp]
-theorem app_closed_iff {p : Program} {f e : Expr} :
+theorem Expr.app_closed_iff {p : Program} {f e : Expr} :
     (f.app e).Closed p ↔ f.Closed p ∧ e.Closed p := by
   constructor
   · intro h
@@ -110,10 +99,7 @@ theorem app_closed_iff {p : Program} {f e : Expr} :
   · rintro ⟨hf, he⟩ n (- | -) <;> solve_by_elim
 
 @[simp]
-theorem bool_closed (p : Program) (b : Bool) : (Expr.bool b).Closed p := nofun
-
-@[simp]
-theorem cond_closed_iff {p : Program} {c et ef : Expr} :
+theorem Expr.cond_closed_iff {p : Program} {c et ef : Expr} :
     (c.cond et ef).Closed p ↔ c.Closed p ∧ et.Closed p ∧ ef.Closed p := by
   constructor
   · intro h
@@ -121,30 +107,26 @@ theorem cond_closed_iff {p : Program} {c et ef : Expr} :
     and_intros <;> solve_by_elim [condC, condT, condF]
   · rintro ⟨hc, het, hef⟩ n (- | - | -) <;> solve_by_elim
 
-theorem lt_size_of_free {p : Program} {e : Expr} {n : Nat} (hp : p.ValidRefs)
-    (he : e.ValidRefs p) (hf : e.Free p n) : n < p.size := by
+theorem Expr.lt_size_of_free {p : Program} {e : Expr} {n : Nat}
+    (hp : p.ValidRefs) (he : e.ValidRefs p) (hf : e.Free p n) : n < p.size := by
   induction hf with simp_all <;> solve_by_elim
 
-theorem lt_size_left_of_nests {p : Program} {m n : Nat} (hp : p.ValidRefs)
-    (h : m ≻[p] n) : m < p.size := by
-  induction h with solve_by_elim [lt_size_of_free]
+theorem Program.lt_size_left_of_nests {p : Program} {m n : Nat}
+    (hp : p.ValidRefs) (h : m ≻[p] n) : m < p.size := by
+  induction h with solve_by_elim [Expr.lt_size_of_free]
 
-theorem lt_size_right_of_nests {p : Program} {m n : Nat} : n ≻[p] m → m < p.size
+theorem Program.lt_size_right_of_nests {p : Program} {m n : Nat} :
+    n ≻[p] m → m < p.size
   | .free _ hm _ _ => hm
   | .step _ _ hm _ _ _ => hm
 
-theorem lt_size_left_of_nestsEq {p : Program} {m n : Nat} (hp : p.ValidRefs) :
-    m ≽[p] n → m < p.size
+theorem Program.lt_size_left_of_nestsEq {p : Program} {m n : Nat}
+    (hp : p.ValidRefs) : m ≽[p] n → m < p.size
   | .refl h => h
   | .nests _ h => lt_size_left_of_nests hp h
 
-theorem nests_self {p : Program} {n : Nat} :
-    (h : n ≻[p] n) → ∃ m ≠ n, (p.fn[n]'(lt_size_right_of_nests h)).Free p m
-  | .free _ _ hne _ => nomatch hne
-  | .step k _ _ hne hf _ => ⟨k, hne, hf⟩
-
-theorem nests_trans {p : Program} {m n k : Nat} (h : m ≻[p] n) (h' : n ≻[p] k) :
-    m ≻[p] k := by
+theorem Program.nests_trans {p : Program} {m n k : Nat} (h : m ≻[p] n)
+    (h' : n ≻[p] k) : m ≻[p] k := by
   induction h' with apply Nests.step <;> assumption
 
 theorem Program.pathWithout_trans {p : Program} {m n k l : Nat}
