LambdaGraph/Subst.lean
@@ -1,48 +1,6 @@
 import LambdaGraph.Nest
 
 /--
-A mapping from old labels to new labels assigned for substitution.
-
-There is also a mapping that maps the newly assigned labels back to their
-original labels.
--/
-structure LabelMap (p : Program) where
-  fwd : Vector Nat p.size
-  inv : Array (Fin p.size)
-
-open Classical in -- TODO: Remove this by implementing Decidable.
-/-- Returns a label map to use for substitution of the variable `n`. -/
-noncomputable def Program.labelMap (p : Program) (n : Nat) : LabelMap p :=
-  aux 0 (Vector.ofFn Fin.val) #[]
-where
-  aux i map inv :=
-    if h : i < p.size then
-      if n ≻[p] i then
-        aux (i + 1) (map.set i (p.size + inv.size)) (inv.push ⟨i, h⟩)
-      else
-        aux (i + 1) map inv
-    else
-      ⟨map, inv⟩
-
-/--
-Substitutes a value for a variable in an expression.
-
-The expression may include references to functions nested inside the function
-corresponding to the substitution variable. For these functions, new versions
-need to be added to the program, with their bodies substituted in the same way.
-This function does not perform this change to the program, but takes a label map
-mapping function labels to the labels assigned to their substituted versions.
--/
-noncomputable def Expr.subst {p : Program} (e : Expr) (map : LabelMap p)
-    (n : Nat) (v : Expr) : Expr :=
-  match e with
-  | var m => if n = m then v else var (map.fwd[m]?.getD m)
-  | fn m => fn (map.fwd[m]?.getD m)
-  | app f e => (f.subst map n v).app (e.subst map n v)
-  | bool b => bool b
-  | cond c et ef => (c.subst map n v).cond (et.subst map n v) (ef.subst map n v)
-
-/--
 A map specifying how variables should be substituted.
 
 Variables that should remain untouched are simply mapped to themselves.
@@ -121,7 +79,7 @@ program, with their bodies substituted in the same way. In addition to the new
 program and expression, this function returns a new function map to allow
 reusing the newly created functions across subexpressions.
 -/
-noncomputable def Expr.subst' (p : Program) (e : Expr) (vm : VarMap p.size)
+noncomputable def Expr.subst (p : Program) (e : Expr) (vm : VarMap p.size)
     (fm : FunMap p.size) : SubstResult p fm :=
   if ∀ n (_ : n < p.size), e.Free p n → vm[n] = .var n then
     ⟨p, e, fm, Nat.le_refl _, Nat.le_refl _⟩
@@ -145,7 +103,7 @@ noncomputable def Expr.subst' (p : Program) (e : Expr) (vm : VarMap p.size)
             have : 0 < Vector.countP (fun x => decide (x = none)) fm :=
               Vector.countP_pos_iff.mpr ⟨none, Vector.mem_of_getElem ‹fm[m] = none›, rfl⟩
             omega
-          let ⟨p₂, f', fm₂, hsize₂, hum₂⟩ := p.fn[m].subst' p₁ vm₁ fm₁
+          let ⟨p₂, f', fm₂, hsize₂, hum₂⟩ := p.fn[m].subst p₁ vm₁ fm₁
           let p₃ := p₂.setBody m' f'
           let e' := fn m'
           have hsize : p.size ≤ p₂.size := by omega
@@ -156,15 +114,15 @@ noncomputable def Expr.subst' (p : Program) (e : Expr) (vm : VarMap p.size)
       else
         ⟨p, fn m, fm, Nat.le_refl _, Nat.le_refl _⟩
     | app f e =>
-      let ⟨p₁, f', fm₁, hsize₁, hum₁⟩ := f.subst' p vm fm
-      let ⟨p₂, e', fm₂, hsize₂, hum₂⟩ := e.subst' p₁ vm.extend fm₁
+      let ⟨p₁, f', fm₁, hsize₁, hum₁⟩ := f.subst p vm fm
+      let ⟨p₂, e', fm₂, hsize₂, hum₂⟩ := e.subst p₁ vm.extend fm₁
       ⟨p₂, f'.app e', fm₂, by omega, by omega⟩
     | bool b => ⟨p, bool b, fm, Nat.le_refl _, Nat.le_refl _⟩
     | cond c et ef =>
-      let ⟨p₁, c', fm₁, hsize₁, hum₁⟩ := c.subst' p vm fm
+      let ⟨p₁, c', fm₁, hsize₁, hum₁⟩ := c.subst p vm fm
       let vm₁ := vm.extend
-      let ⟨p₂, et', fm₂, hsize₂, hum₂⟩ := et.subst' p₁ vm₁ fm₁
-      let ⟨p₃, ef', fm₃, hsize₃, hum₃⟩ := ef.subst' p₂ vm₁.extend fm₂
+      let ⟨p₂, et', fm₂, hsize₂, hum₂⟩ := et.subst p₁ vm₁ fm₁
+      let ⟨p₃, ef', fm₃, hsize₃, hum₃⟩ := ef.subst p₂ vm₁.extend fm₂
       ⟨p₃, c'.cond et' ef', fm₃, by omega, by omega⟩
 termination_by (fm.unmapped, e)
 decreasing_by
@@ -188,654 +146,63 @@ decreasing_by
     · simp_wf
       omega
 
-/--
-Substitutes a value for a variable in a program.
-
-This creates a new version of each function that depends on `n`, as specified by
-the passed label map.
--/
-noncomputable def Program.subst (p : Program) (map : LabelMap p) (n : Nat)
-    (v : Expr) : Program :=
-  let fnExt : Vector Expr map.inv.size :=
-    ⟨map.inv.map (p.fn[·].subst map n v), by simp⟩
-  let tyExt : Vector Ty map.inv.size :=
-    ⟨map.inv.map (p.ty[·]), by simp⟩
-  { size := _, fn := p.fn ++ fnExt, ty := p.ty ++ tyExt }
-
-/--
-Substitutes a value for a variable in a computation.
-
-This computes the map for translating old labels into new ones and applies the
-substitution to the program and the expression.
--/
+/-- Substitutes a value for a variable in a computation. -/
 noncomputable def Computation.subst (p : Computation) (n : Nat) (v : Expr) :
     Computation :=
-  let map := p.labelMap n
-  ⟨p.toProgram.subst map n v, p.expr.subst map n v⟩
-
-/-- Substitutes a value for a variable in a computation. -/
-noncomputable def Computation.subst' (p : Computation) (n : Nat) (v : Expr) :
-    Computation :=
-  let ⟨p', e', _, _, _⟩ := p.expr.subst' p.toProgram (.mk _ n v) (.mk _)
+  let ⟨p', e', _, _, _⟩ := p.expr.subst p.toProgram (.mk _ n v) (.mk _)
   ⟨p', e'⟩
-
-theorem program_subst_size_le {p : Program} {v : Expr} {n : Nat}
-    {map : LabelMap p} : p.size ≤ (p.subst map n v).size := by
-  simp [Program.subst]
-
-theorem lt_subst_size {p : Program} (v : Expr) {m n : Nat} (map : LabelMap p)
-    (hm : m < p.size) : m < (p.subst map n v).size :=
-  Nat.lt_of_lt_of_le hm program_subst_size_le
-
-theorem subst_fn_eq_of_lt {p : Program} (v : Expr) {m n : Nat}
-    (map : LabelMap p) (hm : m < p.size) :
-    (p.subst map n v).fn[m]'(lt_subst_size v map hm) = p.fn[m] := by
-  simp [hm, Program.subst]
-
-theorem subst_fn_eq_of_ge {p : Program} (v : Expr) {m n : Nat}
-    (map : LabelMap p) (hm : p.size ≤ m) (hm' : m < p.size + map.inv.size) :
-    (p.subst map n v).fn[m] = p.fn[map.inv[m - p.size]].subst map n v := by
-  simp [hm, Program.subst]
-
-theorem subst_ty_eq {p : Program} (v : Expr) {m n : Nat} (map : LabelMap p)
-    (hm : m < p.size) :
-    (p.subst map n v).ty[m]'(lt_subst_size v map hm) = p.ty[m] := by
-  simp [hm, Program.subst]
-
-theorem expr_types_in_subst {p : Program} {e : Expr} (v : Expr) {t : Ty}
-    (n : Nat) (map : LabelMap p) (ht : p ⊢ e : t) :
-    p.subst map n v ⊢ e : t := by
-  induction ht with try constructor <;> assumption
-  | var m hm =>
-    rw [← subst_ty_eq v map hm]
-    constructor
-  | fn m hm =>
-    rw [← subst_ty_eq v map hm]
-    constructor
-
-structure LabelMap.ValidNew {p : Program} (map : LabelMap p) {i : Nat}
-    (h : i < p.size) : Prop where
-  fwd_ge : p.size ≤ map.fwd[i]
-  fwd_lt : map.fwd[i] < p.size + map.inv.size
-  inv_fwd_sub : map.inv[map.fwd[i] - p.size] = i
-
-structure LabelMap.Valid {p : Program} (map : LabelMap p) (n : Nat) : Prop where
-  lt : n < p.size
-  not_nests : ∀ {i} (h : i < p.size), n ⊁[p] i → map.fwd[i] = i
-  nests : ∀ {i} (h : i < p.size), n ≻[p] i → map.ValidNew h
-  fwd_inv : ∀ {k} (h : k < map.inv.size), map.fwd[map.inv[k]] = p.size + k
-
-theorem LabelMap.Valid.eq_or_new {p : Program} {map : LabelMap p} {n : Nat}
-    (hmap : map.Valid n) {i : Nat} (hi : i < p.size) :
-    map.fwd[i] = i ∨ map.ValidNew hi := by
-  by_cases h : n ≻[p] i
-  · right
-    exact hmap.nests hi h
-  · left
-    exact hmap.not_nests hi h
-
-theorem LabelMap.Valid.fwd_lt {p : Program} {map : LabelMap p} {n : Nat}
-    (hmap : map.Valid n) {i : Nat} (hi : i < p.size) :
-    map.fwd[i] < p.size + map.inv.size := by
-  rcases hmap.eq_or_new hi with h | h
-  · rw [h]
-    omega
-  · exact h.fwd_lt
-
-theorem LabelMap.Valid.fwd_inj {p : Program} {map : LabelMap p} {n : Nat}
-    (hmap : map.Valid n) {i j : Nat} (hi : i < p.size) (hj : j < p.size)
-    (h : map.fwd[i] = map.fwd[j]) : i = j := by
-  by_cases hni : n ≻[p] i
-  · obtain ⟨hi', hi'', hinvi⟩ := hmap.nests hi hni
-    by_cases hnj : n ≻[p] j
-    · obtain ⟨hj', hj'', hinvj⟩ := hmap.nests hj hnj
-      simp only [h] at hinvi
-      rw [← hinvj, hinvi]
-    · have hj' := hmap.not_nests hj hnj
-      omega
-  · have hi' := hmap.not_nests hi hni
-    by_cases hnj : n ≻[p] j
-    · obtain ⟨hj', hj'', hinvj⟩ := hmap.nests hj hnj
-      omega
-    · have hj' := hmap.not_nests hj hnj
-      rw [← hi', h, hj']
-
-theorem LabelMap.Valid.eq_map_of_ge {p : Program} {map : LabelMap p} {n : Nat}
-    (hmap : map.Valid n) {m : Nat} (hm : p.size ≤ m)
-    (hm' : m < p.size + map.inv.size) : ∃ i : Fin p.size, m = map.fwd[i] := by
-  exists map.inv[m - p.size]
-  rw [hmap.fwd_inv]
-  omega
-
-theorem labelMap_valid (p : Program) {n : Nat} (hn : n < p.size) :
-    (p.labelMap n).Valid n where
-  lt := hn
-  not_nests := by
-    intro i hi h
-    unfold Program.labelMap
-    simp [aux_le_not_nests hi (Nat.zero_le i) h]
-  nests := by
-    intro i hi h
-    unfold Program.labelMap
-    exact aux_le_nests hi (Nat.zero_le i) h
-  fwd_inv := by
-    intro i hi
-    unfold Program.labelMap
-    apply aux_fwd_inv
-    simp
-where
-  aux_gt_map {i j fwd inv} (hi : i < p.size) (hj : i < j) :
-      (Program.labelMap.aux p n j fwd inv).fwd[i] = fwd[i] := by
-    have (eq := hd) d := p.size - j
-    induction d generalizing j fwd inv with unfold Program.labelMap.aux
-    | zero => simp [show ¬j < p.size by omega]
-    | succ d ih =>
-      split
-      · split
-        · have : fwd[i] = (fwd.set j (p.size + inv.size) ‹j < p.size›)[i] := by
-            simp [show j ≠ i by omega]
-          rw [this]
-          apply ih <;> omega
-        · apply ih <;> omega
-      · simp
-  aux_inv_size_ge {j fwd inv} :
-      inv.size ≤ (Program.labelMap.aux p n j fwd inv).inv.size := by
-    have (eq := hd) d := p.size - j
-    induction d generalizing j fwd inv with unfold Program.labelMap.aux
-    | zero => simp [show ¬j < p.size by omega]
-    | succ d ih =>
-      have hj : j < p.size := by omega
-      simp only [hj, ↓reduceDIte, ge_iff_le]
-      split
-      · have hle : inv.size ≤ (inv.push ⟨j, hj⟩).size := by simp
-        apply Nat.le_trans hle
-        apply ih
-        omega
-      · apply ih
-        omega
-  aux_gt_inv {j k fwd inv} (hk : k < inv.size)
-      (hk' : k < (Program.labelMap.aux p n j fwd inv).inv.size) :
-      (Program.labelMap.aux p n j fwd inv).inv[k] = inv[k] := by
-    have (eq := hd) d := p.size - j
-    induction d generalizing j fwd inv with unfold Program.labelMap.aux
-    | zero => simp [show ¬j < p.size by omega]
-    | succ d ih =>
-      have hj : j < p.size := by omega
-      simp [hj]
-      split
-      · have : inv[k] = (inv.push ⟨j, hj⟩)[k]'(by rw [Array.size_push]; omega) :=
-          Eq.symm (Array.getElem_push_lt hk)
-        rw [this]
-        apply ih
-        omega
-      · apply ih
-        omega
-  aux_le_not_nests {i j fwd inv} (hi : i < p.size) (hj : j ≤ i) (h : n ⊁[p] i) :
-      (Program.labelMap.aux p n j fwd inv).fwd[i] = fwd[i] := by
-    have (eq := hd) d := i - j
-    induction d generalizing j fwd inv with unfold Program.labelMap.aux
-    | zero =>
-      simp only [*, show j = i by omega]
-      apply aux_gt_map
-      simp
-    | succ d ih =>
-      have hj' := Nat.lt_of_le_of_lt hj hi
-      simp only [hj', ↓reduceDIte]
-      split
-      · have : fwd[i] = (fwd.set j (p.size + inv.size) hj')[i] := by
-          simp [show j ≠ i by omega]
-        rw [this]
-        apply ih <;> omega
-      · apply ih <;> omega
-  aux_le_nests {i j fwd inv} (hi : i < p.size) (hj : j ≤ i) (h : n ≻[p] i) :
-      (Program.labelMap.aux p n j fwd inv).ValidNew hi := by
-    have (eq := hd) d := i - j
-    induction d generalizing j fwd inv with unfold Program.labelMap.aux
-    | zero =>
-      simp [*, show j = i by omega]
-      refine ⟨?_, ?_, ?_⟩
-      · simp [aux_gt_map]
-      · have hlt : inv.size < (inv.push ⟨i, hi⟩).size := by simp
-        simp only [Nat.lt_add_one, aux_gt_map, Vector.getElem_set_self,
-          Nat.add_lt_add_iff_left]
-        apply Nat.lt_of_lt_of_le hlt
-        simp only [aux_inv_size_ge]
-      · simp only [Nat.lt_add_one, aux_gt_map, Vector.getElem_set_self,
-          Nat.add_sub_cancel_left]
-        have : i = (inv.push ⟨i, hi⟩)[inv.size] := by simp
-        conv => rhs; rw [this]
-        rw [aux_gt_inv]
-    | succ d ih =>
-      have hj' : j < p.size := by omega
-      simp [hj']
-      split <;> apply ih <;> omega
-  aux_fwd_inv {j fwd inv}
-      (h : ∀ k (_ : k < inv.size), ↑inv[k] < j ∧ fwd[inv[k]] = p.size + k) :
-      let ⟨fwd', inv'⟩ := Program.labelMap.aux p n j fwd inv
-      ∀ k (_ : k < inv'.size), fwd'[inv'[k]] = p.size + k := by
-    intro k hk
-    have (eq := hd) d := p.size - j
-    induction d generalizing j fwd inv with unfold Program.labelMap.aux
-    | zero => simp [*, show ¬j < p.size by omega]
-    | succ d ih =>
-      simp only [show j < p.size by omega, ↓reduceDIte, Fin.getElem_fin]
-      split
-      · apply ih
-        · intro k' hk'
-          simp only [Array.size_push] at hk'
-          by_cases k' = inv.size
-          · simp [*]
-          · have : k' < inv.size := by omega
-            obtain ⟨hlt, heq⟩ := h k' this
-            simp only [Fin.getElem_fin] at heq
-            have hne : j ≠ ↑inv[k'] := Ne.symm (Nat.ne_of_lt hlt)
-            simp [*, Array.getElem_push_lt, Nat.lt_succ_of_lt]
-        · omega
-      · apply ih
-        · intro k' hk'
-          obtain ⟨hlt, heq⟩ := h k' hk'
-          simp [*, Nat.lt_succ_of_lt]
-        · omega
-
-theorem subst_ty_map_eq {p : Program} {v : Expr} {m n : Nat} {map : LabelMap p}
-    (hm : m < p.size) (hmap : map.Valid n) :
-    (p.subst map n v).ty[map.fwd[m]]'(hmap.fwd_lt hm) = p.ty[m] := by
-  rcases hmap.eq_or_new hm with h | ⟨hle, hlt, hinv⟩
-  · simp [h, hm, Program.subst]
-  · simp [*, Program.subst]
-
-theorem expr_subst_types {p : Program} {e v : Expr} {t : Ty} {n : Nat}
-    {map : LabelMap p} (hmap : map.Valid n) (ht : p ⊢ e : t)
-    (htv : p ⊢ v : p.ty[n]'hmap.lt) :
-    p.subst map n v ⊢ e.subst map n v : t := by
-  induction ht with try constructor <;> assumption
-  | var m hm =>
-    by_cases hnm : n = m
-    · subst m
-      simp [Expr.subst]
-      exact expr_types_in_subst _ _ _ htv
-    · have hm' : m < map.fwd.size := hm
-      simp [hnm, hm', Expr.subst]
-      rw [← subst_ty_map_eq hm hmap]
-      constructor
-  | fn m hm =>
-    simp only [Expr.subst, hm, getElem?_pos, Option.getD_some]
-    rw [← subst_ty_map_eq hm hmap]
-    constructor
-
-theorem subst_types {p : Program} {e v : Expr} {t : Ty} {n : Nat}
-    (hn : n < p.size) (ht : ⊢ ⟨p, e⟩ : t) (htv : p ⊢ v : p.ty[n]) :
-    ⊢ Computation.subst ⟨p, e⟩ n v : t := by
-  obtain ⟨htp, ht⟩ := ht
-  dsimp only at *
-  constructor
-  · intro m hm
-    simp [Program.subst, Computation.subst]
-    by_cases hm' : m < p.size
-    · simp [hm']
-      exact expr_types_in_subst _ _ _ (htp _)
-    · simp at hm'
-      simp [hm']
-      exact expr_subst_types (labelMap_valid _ hn) (htp _) htv
-  · exact expr_subst_types (labelMap_valid _ hn) ht htv
-
-theorem validRefs_in_subst {p : Program} {e v : Expr} {n : Nat}
-    {map : LabelMap p} (he : e.ValidRefs p) :
-    e.ValidRefs (p.subst map n v) :=
-  Expr.validRefs_of_size_ge program_subst_size_le he
-
-theorem expr_subst_validRefs {p : Program} {e v : Expr} {n : Nat}
-    {map : LabelMap p} (hmap : map.Valid n) (he : e.ValidRefs p)
-    (hv : v.ValidRefs p) : (e.subst map n v).ValidRefs (p.subst map n v) := by
-  induction e with
-    try solve | simp_all [Expr.subst]
-  | var m =>
-    by_cases h : n = m
-    · simp only [Expr.subst, ↓reduceIte, h]
-      exact validRefs_in_subst hv
-    · simp only [Expr.validRefs_var_iff] at he
-      simp [*, Expr.subst, ↓reduceIte, getElem?_pos, Option.getD_some]
-      exact hmap.fwd_lt he
-  | fn m =>
-    simp only [Expr.validRefs_fn_iff] at he
-    simp only [Expr.subst, getElem?_pos, Option.getD_some, Expr.validRefs_fn_iff, he]
-    exact hmap.fwd_lt he
-
-theorem subst_validRefs {p : Program} {v : Expr} {n : Nat} {map : LabelMap p}
-    (hmap : map.Valid n) (hp : p.ValidRefs) (hv : v.ValidRefs p) :
-    (p.subst map n v).ValidRefs := by
-  intro i hi'
-  by_cases hi : i < p.size
-  · simp [*, subst_fn_eq_of_lt]
-    apply_rules [validRefs_in_subst]
-  · simp only [Nat.not_lt] at hi
-    rw [subst_fn_eq_of_ge _ _ hi]
-    apply expr_subst_validRefs <;> apply_rules
-
-theorem subst_eq_var {p : Program} {e v : Expr} {m n : Nat}
-    {map : LabelMap p} (he : e.ValidRefs p) (hv : v.Value)
-    (h : e.subst map n v = .var m) :
-    ∃ i : Fin p.size, m = map.fwd[i] ∧ e = .var i := by
-  cases e with simp only [Expr.subst] at h <;> try contradiction
-  | var k =>
-    simp only [Expr.validRefs_var_iff] at he
-    by_cases hnk : n = k
-    · simp only [hnk, ↓reduceIte] at h
-      subst v
-      nomatch hv
-    · exists ⟨k, he⟩
-      simpa [hnk, he, eq_comm] using h
-
-theorem subst_ne_subst_var {p : Program} {e v : Expr} {n : Nat}
-    {map : LabelMap p} (hmap : map.Valid n) (hv : v.Value) :
-    e.subst map n v ≠ .var n := by
-  cases e with simp only [Expr.subst] <;> try intro; contradiction
-  | var m =>
-    split
-    · intro rfl
-      nomatch hv
-    · by_cases hm : m < p.size
-      · rcases hmap.eq_or_new hm with hm | ⟨hle, hlt, hinv⟩
-        · simp [*, Ne.symm]
-        · simp [hm]
-          intro h
-          rw [h] at hle
-          have := hmap.lt
-          omega
-      · simp [*, Ne.symm]
-
-theorem subst_eq_fn {p : Program} {e v : Expr} {m n : Nat} {map : LabelMap p}
-    (he : e.ValidRefs p) (h : e.subst map n v = .fn m) :
-    e = .var n ∨ ∃ i : Fin p.size, m = map.fwd[i] ∧ e = .fn i := by
-  cases e with simp only [Expr.subst] at h <;> try contradiction
-  | var k =>
-    split at h
-    · simp [*]
-    · simp at h
-  | fn k =>
-    right
-    simp only [Expr.validRefs_fn_iff] at he
-    exists ⟨k, he⟩
-    simpa [he, eq_comm] using h
-
-theorem subst_eq_app {p : Program} {e e₁ e₂ v : Expr} {n : Nat}
-    {map : LabelMap p} (hv : v.Value) (h : e.subst map n v = e₁.app e₂) :
-    ∃ e₁' e₂' : Expr, e = e₁'.app e₂' := by
-  cases e with try solve | simp [Expr.subst] at h
-  | var m =>
-    by_cases hnm : n = m
-    · simp only [Expr.subst, hnm, ↓reduceIte] at h
-      subst v
-      nomatch hv
-    · simp [hnm, Expr.subst] at h
-  | app e₁' e₂' =>
-    simp only [Expr.subst, Expr.app.injEq] at h
-    exists e₁', e₂'
-
-theorem subst_eq_cond {p : Program} {e c et ef v : Expr} {n : Nat}
-    {map : LabelMap p} (hv : v.Value) (h : e.subst map n v = c.cond et ef) :
-    ∃ c' et' ef' : Expr, e = c'.cond et' ef' := by
-  cases e with try solve | simp [Expr.subst] at h
-  | var m =>
-    by_cases hnm : n = m
-    · simp only [Expr.subst, hnm, ↓reduceIte] at h
-      subst v
-      nomatch hv
-    · simp [hnm, Expr.subst] at h
-  | cond c' et' ef' =>
-    simp only [Expr.subst, Expr.cond.injEq] at h
-    exists c', et', ef'
-
-theorem free_of_free_in_subst {p : Program} {e v : Expr} {m n : Nat}
-    {map : LabelMap p} (hp : p.ValidRefs) (he : e.ValidRefs p)
-    (hf : e.Free (p.subst map n v) m) : e.Free p m := by
-  generalize hp' : p.subst map n v = p' at hf
-  open Expr.Free in
-  induction hf with
-    try solve | grind [var, appL, appR, condC, condT, condF]
-  | fn k hk' hne hf ih =>
-    simp only [Expr.validRefs_fn_iff] at he
-    constructor
-    · exact hne
-    · subst p'
-      rw [subst_fn_eq_of_lt _ _ he] at ih
-      exact ih (hp he)
-
-theorem not_free_in_subst {p : Program} {e v : Expr} {n : Nat}
-    {map : LabelMap p} (hmap : map.Valid n) (hp : p.ValidRefs)
-    (he : e.ValidRefs p) (hv : v.ValidRefs p) (hc : v.Closed p) (hvv : v.Value)
-    : ¬(e.subst map n v).Free (p.subst map n v) n := by
-  intro hf
-  generalize hp' : p.subst map n v = p', he' : e.subst map n v = e' at hf
-  induction hf generalizing e with
-  | var => exact subst_ne_subst_var hmap hvv he'
-  | fn m hm' hne hf ih =>
-    subst p'
-    rcases subst_eq_fn he he' with rfl | ⟨⟨i, hi⟩, rfl, rfl⟩
-    · simp only [Expr.subst, ↓reduceIte] at he'
-      subst v
-      simp only [Expr.validRefs_fn_iff] at hv
-      rw [subst_fn_eq_of_lt _ _ hv] at hf
-      replace hf := free_of_free_in_subst hp (hp hv) hf
-      exact hc n (.fn _ _ hne hf)
-    · by_cases hd : n ≻[p] i
-      · obtain ⟨hle, hlt, hinv⟩ := hmap.nests hi hd
-        exact ih (hp hi) (by simp [*, Program.subst])
-      · have hi' := hmap.not_nests hi hd
-        simp only [Fin.getElem_fin, hi', subst_fn_eq_of_lt _ _ hi] at hf
-        simp only [Fin.getElem_fin, hi', ne_eq] at hne
-        replace hf := free_of_free_in_subst hp (hp hi) hf
-        exact hd (.free _ _ hne hf)
-  | appL => grind [Expr.subst, subst_eq_app]
-  | appR => grind [Expr.subst, subst_eq_app]
-  | condC => grind [Expr.subst, subst_eq_cond]
-  | condT => grind [Expr.subst, subst_eq_cond]
-  | condF => grind [Expr.subst, subst_eq_cond]
-
-theorem free_or_eq_map_of_free_in_subst {p : Program} {e v : Expr} {m n : Nat}
-    {map : LabelMap p} (hmap : map.Valid n) (hp : p.ValidRefs)
-    (he : e.ValidRefs p) (hv : v.ValidRefs p) (hvv : v.Value)
-    (hf : (e.subst map n v).Free (p.subst map n v) m) :
-    v.Free p m ∨ ∃ i : Fin p.size, m = map.fwd[i] ∧ e.Free p i := by
-  generalize hp' : p.subst map n v = p', he' : e.subst map n v = e' at hf
-  induction hf generalizing e with
-  | var =>
-    right
-    obtain ⟨⟨i, hi⟩, rfl, rfl⟩ := subst_eq_var he hvv he'
-    exists ⟨i, hi⟩
-    simp [Expr.Free.var]
-  | fn k hk' hne hf ih =>
-    subst p'
-    rcases subst_eq_fn he he' with rfl | ⟨⟨i, hi⟩, rfl, rfl⟩
-    · simp only [Expr.subst, ↓reduceIte] at he'
-      subst v
-      simp only [Expr.validRefs_fn_iff] at hv
-      rw [subst_fn_eq_of_lt _ _ hv] at hf
-      replace hf := free_of_free_in_subst hp (hp hv) hf
-      solve_by_elim
-    · by_cases hd : n ≻[p] i
-      · obtain ⟨hle, hlt, hinv⟩ := hmap.nests hi hd
-        obtain hf' | ⟨j, rfl, hj⟩ := ih (hp hi) (by simp [*, Program.subst])
-        · exact Or.inl hf'
-        · have hij : j ≠ i := by
-            intro rfl
-            contradiction
-          exact Or.inr ⟨j, rfl, .fn _ hi hij hj⟩
-      · obtain hi' := hmap.not_nests hi hd
-        simp only [Fin.getElem_fin, hi', subst_fn_eq_of_lt v map hi] at hf
-        replace hf := free_of_free_in_subst hp (hp hi) hf
-        simp [hi'] at hne
-        have hm : n ⊁[p] m := fun h => hd (.step _ _ hi hne hf h)
-        have hlt := lt_size_of_free hp (hp hi) hf
-        have hm' := hmap.not_nests hlt hm
-        refine Or.inr ⟨⟨m, hlt⟩, by simp [hm'], .fn _ hi hne hf⟩
-  | appL => grind [Expr.subst, Expr.Free.appL, subst_eq_app]
-  | appR => grind [Expr.subst, Expr.Free.appR, subst_eq_app]
-  | condC => grind [Expr.subst, Expr.Free.condC, subst_eq_cond]
-  | condT => grind [Expr.subst, Expr.Free.condT, subst_eq_cond]
-  | condF => grind [Expr.subst, Expr.Free.condF, subst_eq_cond]
-
-theorem eq_map_of_free_in_subst_of_closed {p : Program} {e v : Expr} {m n : Nat}
-    {map : LabelMap p} (hmap : map.Valid n) (hp : p.ValidRefs)
-    (he : e.ValidRefs p) (hv : v.ValidRefs p) (hc : v.Closed p)
-    (hvv : v.Value) (hf : (e.subst map n v).Free (p.subst map n v) m) :
-    ∃ i : Fin p.size, m = map.fwd[i] ∧ e.Free p i :=
-  (free_or_eq_map_of_free_in_subst hmap hp he hv hvv hf).resolve_left (hc m)
-
-theorem nests_of_nests_in_subst {p : Program} {m n k : Nat} {v : Expr}
-    {map : LabelMap p} (hk : k < p.size) (hp : p.ValidRefs)
-    (h : m ≻[p.subst map n v] k) : m < p.size ∧ m ≻[p] k := by
-  generalize hp' : p.subst map n v = p' at h
-  induction h with
-  | free k hk' hne hf' =>
-    have hf : p.fn[k].Free p m := by
-      apply free_of_free_in_subst hp (hp hk)
-      subst p'
-      simpa [subst_fn_eq_of_lt _ _ hk] using hf'
-    constructor
-    · exact lt_size_of_free hp (hp hk) hf
-    · apply Nests.free _ hk hne
-      exact hf
-  | step l k hk' hne hf' h ih =>
-    have hf : p.fn[k].Free p l := by
-      apply free_of_free_in_subst hp (hp hk)
-      subst p'
-      simpa [subst_fn_eq_of_lt _ _ hk] using hf'
-    obtain ⟨hm, ih⟩ := ih (lt_size_of_free hp (hp hk) hf)
-    constructor
-    · exact hm
-    · refine Nests.step _ _ hk hne ?_ ih
-      exact hf
-
-theorem nestsEq_or_nests_of_nests_map_in_subst {p : Program} {m n k : Nat}
-    {v : Expr} {map : LabelMap p} (hk : k < p.size) (hmap : map.Valid n)
-    (hp : p.ValidRefs) (hv : v.ValidRefs p) (hvv : v.Value)
-    (h : m ≻[p.subst map n v] map.fwd[k]) :
-    (∃ l, v.Free p l ∧ m ≽[p] l) ∨
-      ∃ i : Fin p.size, m = map.fwd[i] ∧ i ≻[p] k := by
-  generalize hp' : p.subst map n v = p', hleq : map.fwd[k] = l at h
-  induction h generalizing k with
-  | free k' hk' hne hf' =>
-    by_cases hnk : n ≻[p] k
-    · subst p' k'
-      obtain ⟨hle, hlt, hinv⟩ := hmap.nests hk hnk
-      simp only [subst_fn_eq_of_ge, Fin.getElem_fin, hle, hinv] at hf'
-      obtain hf | ⟨i, heq, hf⟩ :=
-        free_or_eq_map_of_free_in_subst hmap hp (hp _) hv hvv hf'
-      · exact Or.inl ⟨m, hf, .refl (lt_size_of_free hp hv hf)⟩
-      · refine Or.inr ⟨i, heq, ?_⟩
-        have : i ≠ k := by
-          intro h
-          subst k
-          contradiction
-        constructor <;> assumption
-    · subst p' k'
-      simp only [hmap.not_nests hk hnk] at *
-      simp only [subst_fn_eq_of_lt, hk] at hf'
-      have hf := free_of_free_in_subst hp (hp hk) hf'
-      have hm := lt_size_of_free hp (hp hk) hf
-      have hnm : n ⊁[p] m := fun h => hnk (Nests.step _ _ _ hne hf h)
-      refine Or.inr ⟨⟨m, hm⟩, (hmap.not_nests hm hnm).symm, ?_⟩
-      constructor <;> assumption
-  | step l' k' hk' hne hf' h' ih =>
-    by_cases hnk : n ≻[p] k
-    · subst p' k'
-      obtain ⟨hle, hlt, hinv⟩ := hmap.nests hk hnk
-      simp only [subst_fn_eq_of_ge, Fin.getElem_fin, hle, hinv] at hf'
-      obtain hf | ⟨l, heq, hf⟩ :=
-        free_or_eq_map_of_free_in_subst hmap hp (hp _) hv hvv hf'
-      · have hl' := lt_size_of_free hp hv hf
-        have ⟨hm, h⟩ := nests_of_nests_in_subst hl' hp h'
-        exact Or.inl ⟨l', hf, .nests _ h⟩
-      · obtain hf'' | ⟨i, heq', hil⟩ := ih _ heq.symm
-        · exact Or.inl hf''
-        · refine Or.inr ⟨i, heq', ?_⟩
-          have : l ≠ k := by
-            intro h
-            subst k
-            contradiction
-          apply Nests.step <;> assumption
-    · subst p' k'
-      simp only [hmap.not_nests hk hnk] at *
-      simp only [subst_fn_eq_of_lt, hk] at hf'
-      have hf := free_of_free_in_subst hp (hp hk) hf'
-      have hl := lt_size_of_free hp (hp hk) hf
-      obtain ⟨hm, hml⟩ := nests_of_nests_in_subst hl hp h'
-      have hlk : l' ≻[p] k := by constructor <;> assumption
-      have hnl : n ⊁[p] l' := fun h => hnk (nests_trans h hlk)
-      have hnm : n ⊁[p] m := fun h => hnl (nests_trans h hml)
-      exact Or.inr ⟨⟨m, hm⟩, (hmap.not_nests hm hnm).symm, nests_trans hml hlk⟩
-
-theorem subst_wf  {p : Program} {n : Nat} {v : Expr} {map : LabelMap p}
-    (hmap : map.Valid n) (hp : p.ValidRefs) (hv : v.ValidRefs p) (hvv : v.Value)
-    (hwf : p.WF) : (p.subst map n v).WF := by
-  intro m h
-  by_cases hm : m < p.size
-  · obtain ⟨-, h'⟩ := nests_of_nests_in_subst hm hp h
-    exact hwf h'
-  · simp only [Nat.not_lt] at hm
-    have hp' : (p.subst map n v).ValidRefs := subst_validRefs hmap hp hv
-    have hm' := lt_size_left_of_nests hp' h
-    obtain ⟨⟨i, hi⟩, heq⟩ := hmap.eq_map_of_ge hm hm'
-    rw [heq] at h
-    obtain ⟨l, hf, hl⟩ | ⟨⟨j, hj⟩, heq, h'⟩ :=
-      nestsEq_or_nests_of_nests_map_in_subst hi hmap hp hv hvv h
-    · have := lt_size_left_of_nestsEq hp hl
-      omega
-    · simp only [hmap.fwd_inj hi hj heq] at h'
-      exact hwf h'
 
 theorem Program.subst_ty_eq_of_lt {p : Program} {e : Expr} {vm : VarMap p.size}
     {fm : FunMap p.size} {n : Nat} (hn : n < p.size) :
-    let ⟨p', _, fm', hsize, _⟩ := e.subst' p vm fm
+    let ⟨p', _, fm', hsize, _⟩ := e.subst p vm fm
     p'.ty[n] = p.ty[n] := by
-  fun_induction Expr.subst' <;> dsimp only at *
+  fun_induction Expr.subst <;> dsimp only at *
   next p vm fm m hm f m' vm₁ fm₁ p₁ hsize₁ hum₁ p₂ f' fm₂ hsize₂ hum₂ hs₂
       p₃ f'' hsize hum h ih =>
-    have hp₂ : p₂ = (p.fn[m].subst' p₁ vm₁ fm₁).program := by grind
+    have hp₂ : p₂ = (p.fn[m].subst p₁ vm₁ fm₁).program := by grind
     subst p₂
     grind
   next p vm fm f e p₁ f' fm₁ hsize₁ hum₁ hs₁ p₂ e' fm₂ hsize₂ hum₂ hs₂ h ihf ihe =>
-    have hp₁ : p₁ = (f.subst' p vm fm).program := by grind
-    have hp₂ : p₂ = (e.subst' p₁ vm.extend fm₁).program := by grind
+    have hp₁ : p₁ = (f.subst p vm fm).program := by grind
+    have hp₂ : p₂ = (e.subst p₁ vm.extend fm₁).program := by grind
     subst p₁ p₂
     grind
   next p vm fm c et ef p₁ c' fm₁ hsize₁ hum₁ hs₁ vm₁ p₂ et' fm₂ hsize₂ hum₂ hs₂
       p₃ ef' fm₃ hsize₃ hum₃ hs₃ h ihc ihet ihef =>
-    have hp₁ : p₁ = (c.subst' p vm fm).program := by grind
-    have hp₂ : p₂ = (et.subst' p₁ vm.extend fm₁).program := by grind
-    have hp₃ : p₃ = (ef.subst' p₂ vm₁.extend fm₂).program := by grind
+    have hp₁ : p₁ = (c.subst p vm fm).program := by grind
+    have hp₂ : p₂ = (et.subst p₁ vm.extend fm₁).program := by grind
+    have hp₃ : p₃ = (ef.subst p₂ vm₁.extend fm₂).program := by grind
     subst p₁ p₂ p₃
     grind
 
 theorem Program.subst_fn_eq_of_lt {p : Program} {e : Expr} {vm : VarMap p.size}
     {fm : FunMap p.size} {n : Nat} (hn : n < p.size) :
-    let ⟨p', _, _, hsize, _⟩ := (e.subst' p vm fm)
+    let ⟨p', _, _, hsize, _⟩ := (e.subst p vm fm)
     p'.fn[n] = p.fn[n] := by
-  fun_induction Expr.subst' <;>
+  fun_induction Expr.subst <;>
     first | grind
           | dsimp only at *
   next p vm fm m hm f m' vm₁ fm₁ p₁ hsize₁ hum₁ p₂ f' fm₂ hsize₂ hum₂ hs₂
       p₃ f'' hsize hum h ih =>
-    have hp₂ : p₂ = (p.fn[m].subst' p₁ vm₁ fm₁).program := by grind
+    have hp₂ : p₂ = (p.fn[m].subst p₁ vm₁ fm₁).program := by grind
     subst p₂
     grind
   next p vm fm f e p₁ f' fm₁ hsize₁ hum₁ hs₁ p₂ e' fm₂ hsize₂ hum₂ hs₂ h ihf ihe =>
-    have hp₁ : p₁ = (f.subst' p vm fm).program := by grind
-    have hp₂ : p₂ = (e.subst' p₁ vm.extend fm₁).program := by grind
+    have hp₁ : p₁ = (f.subst p vm fm).program := by grind
+    have hp₂ : p₂ = (e.subst p₁ vm.extend fm₁).program := by grind
     subst p₁ p₂
     grind
   next p vm fm c et ef p₁ c' fm₁ hsize₁ hum₁ hs₁ vm₁ p₂ et' fm₂ hsize₂ hum₂ hs₂
       p₃ ef' fm₃ hsize₃ hum₃ hs₃ h ihc ihet ihef =>
-    have hp₁ : p₁ = (c.subst' p vm fm).program := by grind
-    have hp₂ : p₂ = (et.subst' p₁ vm.extend fm₁).program := by grind
-    have hp₃ : p₃ = (ef.subst' p₂ vm₁.extend fm₂).program := by grind
+    have hp₁ : p₁ = (c.subst p vm fm).program := by grind
+    have hp₂ : p₂ = (et.subst p₁ vm.extend fm₁).program := by grind
+    have hp₃ : p₃ = (ef.subst p₂ vm₁.extend fm₂).program := by grind
     subst p₁ p₂ p₃
     grind
 
 theorem Expr.types_in_subst_of_types {p : Program} {e₁ e₂ : Expr} {t : Ty}
     {vm : VarMap p.size} {fm : FunMap p.size} (ht : p ⊢ e₁ : t) :
-    (e₂.subst' p vm fm).program ⊢ e₁ : t := by
+    (e₂.subst p vm fm).program ⊢ e₁ : t := by
   induction ht with
     first | constructor <;> assumption
           | rw [← Program.subst_ty_eq_of_lt]; constructor
@@ -925,7 +292,7 @@ theorem update_types {p : Program} {vm : VarMap p.size} {b : Expr} {m : Nat}
 
 theorem extend_types {p : Program} (e : Expr) {vm : VarMap p.size}
     (fm : FunMap p.size) (hvm : vm.Types p) :
-    vm.extend.Types (e.subst' p vm fm).program := by
+    vm.extend.Types (e.subst p vm fm).program := by
   intro i hi
   simp only [VarMap.extend, Fin.getElem_fin, Vector.getElem_ofFn]
   split
@@ -986,17 +353,17 @@ theorem update_types {p : Program} {fm : FunMap p.size} {b : Expr} {m : Nat}
 
 theorem subst_types {p : Program} {e : Expr} {vm : VarMap p.size}
     {fm : FunMap p.size} (hfm : fm.Types p) :
-    let ⟨p', _, fm', _, _⟩ := e.subst' p vm fm
+    let ⟨p', _, fm', _, _⟩ := e.subst p vm fm
     fm'.Types p' := by
   dsimp only
-  fun_induction Expr.subst' <;>
+  fun_induction Expr.subst <;>
     first | grind
           | dsimp only at *
   next p vm fm m hm f m' vm₁ fm₁ p₁ hsize₁ hum₁ p₂ f' fm₂ hsize₂ hum₂ hs₂
       p₃ f'' hsize hum h ih =>
-    have hp₂ : p₂ = (p.fn[m].subst' p₁ vm₁ fm₁).program := by grind
+    have hp₂ : p₂ = (p.fn[m].subst p₁ vm₁ fm₁).program := by grind
     subst p₂
-    have hfm₂ : fm₂ = (p.fn[m].subst' p₁ vm₁ fm₁).funMap := by grind
+    have hfm₂ : fm₂ = (p.fn[m].subst p₁ vm₁ fm₁).funMap := by grind
     subst fm₂
     apply ih
     intro i hi k hk
@@ -1017,9 +384,9 @@ end FunMap
 
 theorem Expr.subst_types {p : Program} {e : Expr} {t : Ty} {vm : VarMap p.size}
     {fm : FunMap p.size} (ht : p ⊢ e : t) (hvm : vm.Types p) (hfm : fm.Types p) :
-    let ⟨p', e', _, _, _⟩ := e.subst' p vm fm
+    let ⟨p', e', _, _, _⟩ := e.subst p vm fm
     p' ⊢ e' : t := by
-  fun_induction subst' generalizing t <;> dsimp only at *
+  fun_induction subst generalizing t <;> dsimp only at *
   next => exact ht
   next p vm fm m h =>
     by_cases hm : m < p.size
@@ -1030,7 +397,7 @@ theorem Expr.subst_types {p : Program} {e : Expr} {t : Ty} {vm : VarMap p.size}
   next p vm fm m hm f m' vm₁ fm₁ p₁ hsize₁ hum₁ p₂ f' fm₂ hsize₂ hum₂ hs₂
       p₃ f'' hsize hum h ih =>
     have .fn _ _ := ht
-    have hp₂ : p₂ = (p.fn[m].subst' p₁ vm₁ fm₁).program := by grind
+    have hp₂ : p₂ = (p.fn[m].subst p₁ vm₁ fm₁).program := by grind
     subst hp₂
     have : p.ty[m] = p₃.ty[p.size] := by grind [Program.subst_ty_eq_of_lt]
     rw [this]
@@ -1053,8 +420,8 @@ theorem Expr.subst_types {p : Program} {e : Expr} {t : Ty} {vm : VarMap p.size}
 
 theorem Program.subst_types {p : Program} {e : Expr} {vm : VarMap p.size}
     {fm : FunMap p.size} (ht : ⊢ p) (hvm : vm.Types p) (hfm : fm.Types p) :
-    ⊢ (e.subst' p vm fm).program := by
-  fun_induction Expr.subst' <;>
+    ⊢ (e.subst p vm fm).program := by
+  fun_induction Expr.subst <;>
     first | grind [VarMap.extend_types, FunMap.subst_types]
           | dsimp only at *
   next p vm fm m hm f m' vm₁ fm₁ p₁ hsize₁ hum₁ p₂ f' fm₂ hsize₂ hum₂ hs₂
@@ -1067,14 +434,14 @@ theorem Program.subst_types {p : Program} {e : Expr} {vm : VarMap p.size}
       · constructor
     have hvm₁ : vm₁.Types p₁ := VarMap.update_types hm hvm
     have hfm₁ : fm₁.Types p₁ := FunMap.update_types hm hfm
-    have hp₂ : p₂ = (p.fn[m].subst' p₁ vm₁ fm₁).program := by grind
+    have hp₂ : p₂ = (p.fn[m].subst p₁ vm₁ fm₁).program := by grind
     subst p₂
     have ht₂ : ⊢ _ := ih ht₁ hvm₁ hfm₁
     intro i hi
     simp only [p₃]
     by_cases m' = i
     · subst i
-      have hf' : f' = (p.fn[m].subst' p₁ vm₁ fm₁).expr := by grind
+      have hf' : f' = (p.fn[m].subst p₁ vm₁ fm₁).expr := by grind
       subst f'
       apply Expr.types_in_setBody_of_types
       simp only [Vector.getElem_set_self]
@@ -1115,8 +482,8 @@ theorem FunMap.extends_update {n : Nat} {fm : FunMap n} {m : Nat} (hm : m < n)
 
 @[grind! .]
 theorem FunMap.extends_subst {p : Program} {e : Expr} {vm : VarMap p.size}
-    {fm : FunMap p.size} : (e.subst' p vm fm).funMap.Extends fm := by
-  fun_induction Expr.subst' <;>
+    {fm : FunMap p.size} : (e.subst p vm fm).funMap.Extends fm := by
+  fun_induction Expr.subst <;>
     try solve | constructor <;> simp_all
               | grind [extends_update]
 
@@ -1325,9 +692,9 @@ theorem Program.validSubst_push_recurse {p : Program} {vm : VarMap p.size}
 theorem Program.validSubst_and_validRefs_and_localProvenance_subst {p : Program}
     {e : Expr} {vm : VarMap p.size} {fm : FunMap p.size}
     (hvalid : p.ValidSubst vm fm) (he : e.ValidRefs p) (hns : e.NoSubst fm) :
-    let ⟨p', e', fm', _, _⟩ := e.subst' p vm fm
+    let ⟨p', e', fm', _, _⟩ := e.subst p vm fm
     p'.ValidSubst vm.extend fm' ∧ e'.ValidRefs p' ∧ fm'.LocalProvenance e e' none := by
-  fun_induction Expr.subst'
+  fun_induction Expr.subst
   next p e vm fm h =>
     simp only [VarMap.extend_eq, true_and, hvalid, he]
     intro n r hn hnn' hl
@@ -1418,7 +785,7 @@ theorem Program.validSubst_and_validRefs_and_localProvenance_subst {p : Program}
           simp only [reduceCtorEq, false_or] at hl
           rw [hfmm] at hnn'
           have heq : p₂.fn[m] = p.fn[m] := by
-            have hp₂ : p₂ = (p.fn[m].subst' p₁ vm₁ fm₁).program := by grind
+            have hp₂ : p₂ = (p.fn[m].subst p₁ vm₁ fm₁).program := by grind
             subst p₂
             rw [subst_fn_eq_of_lt (by lia)]
             simp [p₁, hm]
@@ -1437,7 +804,7 @@ theorem Program.validSubst_and_validRefs_and_localProvenance_subst {p : Program}
         have hnm' : m' ≠ n := by grind [h₂.fm_idem]
         have heq : p₃.fn[n] = p.fn[n] := by
           simp only [ne_eq, not_false_eq_true, Vector.getElem_set_ne, p₃, hnm']
-          have hp₂ : p₂ = (p.fn[m].subst' p₁ vm₁ fm₁).program := by grind
+          have hp₂ : p₂ = (p.fn[m].subst p₁ vm₁ fm₁).program := by grind
           subst p₂
           rw [subst_fn_eq_of_lt (by lia)]
           simp [p₁, *]
@@ -1536,31 +903,31 @@ theorem Program.validSubst_and_validRefs_and_localProvenance_subst {p : Program}
 theorem Program.validSubst_subst {p : Program} {e : Expr} {vm : VarMap p.size}
     {fm : FunMap p.size} (hvalid : p.ValidSubst vm fm) (he : e.ValidRefs p)
     (hns : e.NoSubst fm) :
-    let ⟨p', _, fm', _, _⟩ := e.subst' p vm fm
+    let ⟨p', _, fm', _, _⟩ := e.subst p vm fm
     p'.ValidSubst vm.extend fm' :=
   Program.validSubst_and_validRefs_and_localProvenance_subst hvalid he hns |>.1
 
 theorem Expr.validRefs_subst {p : Program} {e : Expr} {vm : VarMap p.size}
     {fm : FunMap p.size} (hvalid : p.ValidSubst vm fm) (he : e.ValidRefs p)
     (hns : e.NoSubst fm) :
-    let ⟨p', e', _, _, _⟩ := e.subst' p vm fm
+    let ⟨p', e', _, _, _⟩ := e.subst p vm fm
     e'.ValidRefs p' :=
   Program.validSubst_and_validRefs_and_localProvenance_subst hvalid he hns |>.2.1
 
 theorem Expr.localProvenance_subst {p : Program} {e : Expr} {vm : VarMap p.size}
     {fm : FunMap p.size} (hvalid : p.ValidSubst vm fm) (he : e.ValidRefs p)
     (hns : e.NoSubst fm) :
-    let ⟨_, e', fm', _, _⟩ := e.subst' p vm fm
+    let ⟨_, e', fm', _, _⟩ := e.subst p vm fm
     fm'.LocalProvenance e e' none :=
   Program.validSubst_and_validRefs_and_localProvenance_subst hvalid he hns |>.2.2
 
 theorem Program.exists_of_ge_in_subst {p : Program} {e : Expr}
     {vm : VarMap p.size} {fm : FunMap p.size} (h : p.ValidSubst vm fm)
     (he : e.ValidRefs p) (hns : e.NoSubst fm) {n' : Nat} (hn' : p.size ≤ n') :
-    let ⟨p', _, fm', _, _⟩ := e.subst' p vm fm
+    let ⟨p', _, fm', _, _⟩ := e.subst p vm fm
     n' < p'.size → ∃ (n : Nat) (_ : n < p.size), n' = fm'[n].getD n := by
   intro hlt
-  fun_induction Expr.subst' generalizing n' <;> try grind
+  fun_induction Expr.subst generalizing n' <;> try grind
   next p vm fm m hm hfm m' vm₁ fm₁ p₁ hsize₁ hum₁ p₂ f' fm₂ hsize₂ hum₂ hs₂
       p₃ f'' hsize hum h ih =>
     rw [hs₂] at ih
@@ -1579,9 +946,9 @@ theorem Program.exists_of_ge_in_subst {p : Program} {e : Expr}
         simp only [ne_eq, not_false_eq_true, FunMap.getElem_update_ne, fm₁, *] at hl ⊢
         exact h.fn_noSubst hm hfm hn hl
     have h₂ : p₂.ValidSubst vm₁.extend fm₂ := by
-      have hp₂ : p₂ = (p.fn[m].subst' p₁ vm₁ fm₁).program := by grind
+      have hp₂ : p₂ = (p.fn[m].subst p₁ vm₁ fm₁).program := by grind
       subst p₂
-      have hfm₂ : fm₂ = (p.fn[m].subst' p₁ vm₁ fm₁).funMap := by grind
+      have hfm₂ : fm₂ = (p.fn[m].subst p₁ vm₁ fm₁).funMap := by grind
       subst fm₂
       exact validSubst_subst h₁ (Expr.validRefs_in_push (h.validRefs hm)) hns
     by_cases n' = p.size
@@ -1662,7 +1029,7 @@ theorem Program.exists_of_ge_in_subst {p : Program} {e : Expr}
 
 theorem Program.lt_size_of_pathWithout_of_lt {p : Program} {e : Expr}
     {vm : VarMap p.size} {fm : FunMap p.size} (hp : p.ValidRefs) {m n k : Nat}
-    (hm : m < p.size) (hp : m ⟶[(e.subst' p vm fm).program, n]* k) :
+    (hm : m < p.size) (hp : m ⟶[(e.subst p vm fm).program, n]* k) :
     k < p.size := by
   induction hp with
   | refl m hm => exact hm
@@ -1675,15 +1042,15 @@ theorem Program.pathWithout_of_pathWithout_in_subst {p : Program} {e : Expr}
     {vm : VarMap p.size} {fm : FunMap p.size} (h : p.ValidSubst vm fm)
     (he : e.ValidRefs p) (hns : e.NoSubst fm) {n' m' k' : Nat} (hn' : p.size ≤ n')
     (hm' : p.size ≤ m') (hk' : p.size ≤ k') :
-    let ⟨p', _, fm', _, _⟩ := e.subst' p vm fm
+    let ⟨p', _, fm', _, _⟩ := e.subst p vm fm
     n' < p'.size → m' < p'.size → k' < p'.size → m' ⟶[p', n']* k' →
       ∃ (n m k : Nat) (hn : n < p.size) (hm : m < p.size) (hk : k < p.size),
         n' = fm'[n].getD n ∧ m' = fm'[m].getD m ∧ k' = fm'[k].getD k ∧ m ⟶[p, n]* k := by
   intro hnlt hmlt hklt hp'
-  let p' := (e.subst' p vm fm).program
-  let e' := (e.subst' p vm fm).expr
-  let fm' := (e.subst' p vm fm).funMap
-  have hsize := (e.subst' p vm fm).size_ge
+  let p' := (e.subst p vm fm).program
+  let e' := (e.subst p vm fm).expr
+  let fm' := (e.subst p vm fm).funMap
+  have hsize := (e.subst p vm fm).size_ge
   have h' : p'.ValidSubst vm.extend fm' := Program.validSubst_subst h he hns
   induction hp' with
   | refl m' hne' =>
@@ -1715,14 +1082,14 @@ theorem Program.free_in_fn_of_free_in_subst_of_ge {p : Program} {e : Expr}
     {vm : VarMap p.size} {fm : FunMap p.size} (h : p.ValidSubst vm fm)
     (he : e.ValidRefs p) (hns : e.NoSubst fm) {n' m' : Nat} (hn' : p.size ≤ n')
     (hm' : p.size ≤ m') (hne' : n' ≠ m') :
-    let ⟨p', _, fm', _, _⟩ := e.subst' p vm fm
+    let ⟨p', _, fm', _, _⟩ := e.subst p vm fm
     ∀ (_ : m' < p'.size), p'.fn[m'].Free p' n' →
       ∃ (n m : Nat) (hn : n < p.size) (hm : m < p.size),
         n' = fm'[n].getD n ∧ m' = fm'[m].getD m ∧ p.fn[m].Free p n := by
   intro hmlt hf'
-  let p' := (e.subst' p vm fm).program
-  let e' := (e.subst' p vm fm).expr
-  let fm' := (e.subst' p vm fm).funMap
+  let p' := (e.subst p vm fm).program
+  let e' := (e.subst p vm fm).expr
+  let fm' := (e.subst p vm fm).funMap
   have h' : p'.ValidSubst vm.extend fm' := Program.validSubst_subst h he hns
   obtain ⟨k', hklt, hlv', hp'⟩ := (free_in_fn_iff hmlt hne').mp hf'
   have hk' : p.size ≤ k' := by grind [subst_fn_eq_of_lt]
@@ -1740,13 +1107,13 @@ theorem Program.free_in_fn_of_free_in_subst_of_ge {p : Program} {e : Expr}
 theorem Expr.free_of_free_in_subst_of_ge {p : Program} {e : Expr}
     {vm : VarMap p.size} {fm : FunMap p.size} (h : p.ValidSubst vm fm)
     (he : e.ValidRefs p) (hns : e.NoSubst fm) {n' : Nat} (hn' : p.size ≤ n') :
-    let ⟨p', e', fm', _, _⟩ := e.subst' p vm fm
+    let ⟨p', e', fm', _, _⟩ := e.subst p vm fm
     e'.Free p' n' → ∃ (n : Nat) (_ : n < p.size),
       n' = fm'[n].getD n ∧ e.Free p n := by
   intro hf
-  let p' := (e.subst' p vm fm).program
-  let e' := (e.subst' p vm fm).expr
-  let fm' := (e.subst' p vm fm).funMap
+  let p' := (e.subst p vm fm).program
+  let e' := (e.subst p vm fm).expr
+  let fm' := (e.subst p vm fm).funMap
   have h' : p'.ValidSubst vm.extend fm' := Program.validSubst_subst h he hns
   have hlt : n' < p'.size :=
     lt_size_of_free h'.validRefs (validRefs_subst h he hns) hf
@@ -1775,7 +1142,7 @@ theorem Expr.free_of_free_in_subst_of_ge {p : Program} {e : Expr}
 theorem Program.lt_size_of_free_in_subst_of_lt {p : Program} {e : Expr}
     {vm : VarMap p.size} {fm : FunMap p.size} (h : p.ValidRefs)
     {n m : Nat} (hm : m < p.size) (hne : n ≠ m) :
-    let ⟨p', _, _, _, _⟩ := e.subst' p vm fm
+    let ⟨p', _, _, _, _⟩ := e.subst p vm fm
     p'.fn[m].Free p' n → n < p.size := by
   intro hf
   obtain ⟨k, hk, hlv, hp⟩ := (free_in_fn_iff (by lia) hne).mp hf
@@ -1785,7 +1152,7 @@ theorem Program.lt_size_of_free_in_subst_of_lt {p : Program} {e : Expr}
 
 theorem Program.lt_size_of_nests_in_subst_of_lt {p : Program} {e : Expr}
     {vm : VarMap p.size} {fm : FunMap p.size} (h : p.ValidRefs) {n m : Nat}
-    (hm : m < p.size) (hnests : n ≻[(e.subst' p vm fm).program] m) :
+    (hm : m < p.size) (hnests : n ≻[(e.subst p vm fm).program] m) :
     n < p.size := by
   induction hnests with
   | free m hm' hne hf =>
@@ -1795,15 +1162,15 @@ theorem Program.lt_size_of_nests_in_subst_of_lt {p : Program} {e : Expr}
 
 theorem Expr.validRefs_in_subst {p : Program} {e₁ e₂ : Expr}
     {vm : VarMap p.size} {fm : FunMap p.size} (he₁ : e₁.ValidRefs p) :
-    e₁.ValidRefs (e₂.subst' p vm fm).program :=
-  let ⟨_, _, _, hsize, _⟩ := (e₂.subst' p vm fm)
+    e₁.ValidRefs (e₂.subst p vm fm).program :=
+  let ⟨_, _, _, hsize, _⟩ := (e₂.subst p vm fm)
   validRefs_of_size_ge hsize he₁
 
 theorem Expr.free_of_free_in_subst {p : Program} {e₁ e₂ : Expr}
     {vm : VarMap p.size} {fm : FunMap p.size} {n : Nat} (hp : p.ValidRefs)
-    (he₁ : e₁.ValidRefs p) (hf : e₁.Free (e₂.subst' p vm fm).program n) :
+    (he₁ : e₁.ValidRefs p) (hf : e₁.Free (e₂.subst p vm fm).program n) :
     e₁.Free p n := by
-  generalize hp' : (e₂.subst' p vm fm).program = p' at hf
+  generalize hp' : (e₂.subst p vm fm).program = p' at hf
   induction hf with
     try grind [Free.var, Free.appL, Free.appR, Free.condC, Free.condT, Free.condF]
   | fn k hk' hne hf ih =>
@@ -1816,9 +1183,9 @@ theorem Expr.free_of_free_in_subst {p : Program} {e₁ e₂ : Expr}
 
 theorem Program.nests_of_nests_in_subst_of_lt {p : Program} {e : Expr}
     {vm : VarMap p.size} {fm : FunMap p.size} {m n : Nat} (hn : n < p.size)
-    (hp : p.ValidRefs) (h : m ≻[(e.subst' p vm fm).program] n) :
+    (hp : p.ValidRefs) (h : m ≻[(e.subst p vm fm).program] n) :
     m ≻[p] n := by
-  generalize hp' : (e.subst' p vm fm).program = p' at h
+  generalize hp' : (e.subst p vm fm).program = p' at h
   induction h with
   | free n hn' hne hf' =>
     subst p'
@@ -1831,18 +1198,18 @@ theorem Program.nests_of_nests_in_subst_of_lt {p : Program} {e : Expr}
     have hf : p.fn[n].Free p k := by
       apply Expr.free_of_free_in_subst hp (hp hn)
       simpa [subst_fn_eq_of_lt hn] using hf'
-    exact Nests.step _ _ hn hne hf (ih (lt_size_of_free hp (hp hn) hf))
+    exact Nests.step _ _ hn hne hf (ih (Expr.lt_size_of_free hp (hp hn) hf))
 
 theorem Program.nests_of_nests_in_subst_of_ge {p : Program} {e : Expr}
     {vm : VarMap p.size} {fm : FunMap p.size} (h : p.ValidSubst vm fm)
     (he : e.ValidRefs p) (hns : e.NoSubst fm) {n' m' : Nat} (hn' : p.size ≤ n') :
-    let ⟨p', _, fm', _, _⟩ := e.subst' p vm fm
+    let ⟨p', _, fm', _, _⟩ := e.subst p vm fm
     n' ≻[p'] m' → ∃ (n m : Nat) (hn : n < p.size) (hm : m < p.size),
       n' = fm'[n].getD n ∧ m' = fm'[m].getD m ∧ n ≻[p] m := by
   intro hnests'
-  let p' := (e.subst' p vm fm).program
-  let e' := (e.subst' p vm fm).expr
-  let fm' := (e.subst' p vm fm).funMap
+  let p' := (e.subst p vm fm).program
+  let e' := (e.subst p vm fm).expr
+  let fm' := (e.subst p vm fm).funMap
   have h' : p'.ValidSubst vm.extend fm' := Program.validSubst_subst h he hns
   induction hnests' with
   | free m' hltm hne' hf' =>
@@ -1878,7 +1245,7 @@ namespace Computation
 
 theorem subst_types {c : Computation} {t : Ty} {n : Nat} {v : Expr}
     (hn : n < c.size) (ht : ⊢ c : t) (hv : c.toProgram ⊢ v : c.ty[n]) :
-    ⊢ c.subst' n v : t := by
+    ⊢ c.subst n v : t := by
   refine ⟨Program.subst_types ht.program_types ?hvm ?hfm,
           Expr.subst_types ht.expr_types ?hvm ?hfm⟩
   · exact VarMap.mk_types hn hv
@@ -1886,9 +1253,9 @@ theorem subst_types {c : Computation} {t : Ty} {n : Nat} {v : Expr}
 
 theorem subst_wf {c : Computation} {n : Nat} {v : Expr} (hp : c.ValidRefs)
     (he : c.expr.ValidRefs c.toProgram) (hv : v.ValidRefs c.toProgram)
-    (h : c.WF) : (c.subst' n v).WF := by
+    (h : c.WF) : (c.subst n v).WF := by
   let ⟨p, e⟩ := c
-  dsimp only [subst'] at *
+  dsimp only [subst] at *
   intro m hnests
   by_cases hm : m < p.size
   · exact h <| Program.nests_of_nests_in_subst_of_lt hm hp hnests
